Top-level correctness theorem
Moved to own file for clarity.

Squashed commits:

- Clear admits in VerilogEquivalenceCorrectness
- Clear transfer_clean admit
- Clear sort_module_equivalent admit
- WIP clean_module_statically (SEE MESSAGE)

  We need defined inputs -> defined outputs for expressions.

  This is not generally true. There is a number of conditions for
  it (like, "index of bit-selects is statically in-bounds"), which are
  currently checked in expr_to_smt. I think the way to go is to move
  those checks into typechecking and make them part of the expression syntax.

  Then, this lemma will be provable for every constructible expression.
- WIP Add wf conditions to expressions
- WIP Add well-formedness proofs to expression syntax
  As required above - those were originally checked in VerilogToSMT,
  moved the check to typechecking and added the proofs into the
  expression syntax. For bit-selects specifically, this required
  splitting it into two constructors - one for 'correct by width' and
  one for 'correct by literal'.
- WIP ALL DONE!!!!!

bin/driver/VerilogPP.ml
@@ -147,8 +147,10 @@ module Typed = struct
     | Verilog.UnaryOp (_, e) ->
         (* fprintf fmt "( %a@ %a )" unaryop op expression e *)
         fprintf fmt "( +@ %a )" expression e
-    | Verilog.BitSelect (_, _, target, index) ->
+    | Verilog.BitSelect_width (_, _, target, index) ->
         fprintf fmt "%a[%a]" expression target expression index
+    | Verilog.BitSelect_const (_, w_index, target, index) ->
+        fprintf fmt "%a[%a]" expression target expression (Verilog.IntegerLiteral (w_index, index))
     | Verilog.Concatenation (_, _, lhs, rhs) ->
         fprintf fmt "{%a %a}" expression lhs expression rhs
     | Verilog.Conditional (_, _, cond, t, f) ->
