vera/VerilogEquivalence.v
@@ -11,6 +11,7 @@ From vera Require VerilogToSMT.
 From vera Require SMTQueries.
 From vera Require Import Decidable.
 From vera Require Import Tactics.
+From vera Require DropInternal.
 
 From ExtLib Require Import Data.List.
 From ExtLib Require Import Data.Monads.EitherMonad.
@@ -230,9 +231,3 @@ Next Obligation.
   pose proof (verilog_to_smt_max_name TaggedVariable.VerilogLeft) as Hmax_left. insterU Hmax_left.
   lia.
 Qed.
-
-Definition equivalence_query_general (verilog1 verilog2 : Verilog.vmodule) : sum string (SMT.smt_with_namemap) :=
-  let* inlinedVerilog1 := AssignmentForwarding.forward_assignments verilog1 in
-  let* inlinedVerilog2 := AssignmentForwarding.forward_assignments verilog2 in
-  
-  equivalence_query inlinedVerilog1 inlinedVerilog2.
