vera/EquivalenceTop.v
@@ -1,0 +1,222 @@
+From vera Require Import Verilog.
+From vera Require VerilogSemantics.
+Import VerilogSemantics.Sort.
+From vera Require Import VerilogSMT.
+Import (coercions) SMT.
+From vera Require AssignmentForwarding.
+From vera Require DropInternal.
+From vera Require VerilogEquivalence.
+
+From ExtLib Require Import Structures.Monads.
+
+From Stdlib Require Import String.
+
+From Equations Require Import Equations.
+
+Import MonadLetNotation.
+Local Open Scope monad_scope.
+Local Open Scope string.
+
+Definition sort_module (v : Verilog.vmodule) : string + Verilog.vmodule :=
+  let* sorted_body :=
+    match sort_module_items (Verilog.module_inputs v) (Verilog.modBody v) with
+    | None => inl "Module not sortable"
+    | Some sorted => inr sorted
+    end in
+  ret {|
+    Verilog.modName := Verilog.modName v;
+    Verilog.modVariableDecls := Verilog.modVariableDecls v;
+    Verilog.modBody := sorted_body
+  |}.
+
+Definition equivalence_query_general (verilog1 verilog2 : Verilog.vmodule) : sum string (SMT.smt_with_namemap) :=
+  let* sorted1 := sort_module verilog1 in
+  let* inlined1 := AssignmentForwarding.forward_assignments sorted1 in
+  let* internal_dropped1 := DropInternal.drop_internal inlined1 in
+
+  let* sorted2 := sort_module verilog2 in
+  let* inlined2 := AssignmentForwarding.forward_assignments sorted2 in
+  let* internal_dropped2 := DropInternal.drop_internal inlined2 in
+
+  VerilogEquivalence.equivalence_query internal_dropped1 internal_dropped2.
+
+From vera Require Import VerilogSMT.
+From vera Require Import SMTQueries.
+From vera Require Import VerilogSemantics.
+Import CombinationalOnly.
+Import Equivalence.
+Import ExactEquivalence.
+From vera Require Import Common.
+From vera Require Import Tactics.
+From vera Require Import AssignmentForwardingCorrect.
+From vera Require Import VerilogEquivalenceCorrectness.
+
+From Stdlib Require Import Relations.
+From Stdlib Require Import Structures.Equalities.
+From Stdlib Require Import Morphisms.
+From Stdlib Require Import Setoid.
+
+Local Open Scope verilog.
+
+Theorem sort_module_equivalent v1 v2 :
+  sort_module v1 = inr v2 ->
+  v1 ~~~ v2.
+Proof.
+  unfold sort_module. intros H. monad_inv.
+  apply equal_exact_equivalence; try reflexivity; expect 1.
+  unfold run_vmodule. simpl.
+  unfold Verilog.module_inputs in *; simpl in *.
+  intros regs. rewrite E0.
+  rewrite sort_module_items_stable
+    by eauto using sort_module_items_sorted.
+  reflexivity.
+Qed.
+
+Lemma equivalence_query_clean_left v1 v2 smt :
+  VerilogEquivalence.equivalence_query v1 v2 = inr smt ->
+  clean_module v1.
+Proof.
+  intros H.
+  unfold VerilogEquivalence.equivalence_query in H.
+  monad_inv.
+  eapply VerilogEquivalenceCorrectness.verilog_to_smt_clean.
+  eassumption.
+Qed.
+
+Lemma equivalence_query_clean_right v1 v2 smt :
+  VerilogEquivalence.equivalence_query v1 v2 = inr smt ->
+  clean_module v2.
+Proof.
+  intros H.
+  unfold VerilogEquivalence.equivalence_query in H.
+  monad_inv.
+  eapply VerilogEquivalenceCorrectness.verilog_to_smt_clean.
+  eassumption.
+Qed.
+
+Lemma transfer_clean v1 v2 :
+  v1 ~~~ v2 ->
+  clean_module v1 ->
+  clean_module v2.
+Proof.
+  intros [Hinput_names Houtput_names Hequiv].
+  unfold clean_module.
+  rewrite <- Hinput_names, Houtput_names.
+  intros Hclean e Hinputs_defined.
+  specialize (Hclean e Hinputs_defined).
+  destruct Hclean as [e' [Hrun [Hinputs Houtputs_defined]]].
+  specialize (Hequiv e'). destruct Hequiv as [Hequiv _].
+  unfold "⇓" in Hequiv. edestruct Hequiv as [e'' [Hrun'' [Hinputs'' [Houtputs_defined'' Hmatch'']]]]; clear Hequiv. 
+  - exists e'. repeat split.
+    + setoid_rewrite <- Hinputs at 1.
+      apply Hrun.
+    + setoid_rewrite <- Hinputs. 
+      apply VerilogToSMTCorrect.defined_value_for_has_value_for.
+      apply Hinputs_defined.
+    + apply VerilogToSMTCorrect.defined_value_for_has_value_for.
+      rewrite <- Houtput_names in Houtputs_defined.
+      apply Houtputs_defined.
+  - symmetry in Hmatch''.
+    rewrite <- Hinput_names, <- Houtput_names in *.
+    RegisterState.unpack_match_on.
+    exists e''. repeat split.
+    + rewrite Hinputs at 1. apply Hrun''.
+    + transitivity e'; eassumption.
+    + rewrite <- H0. apply Houtputs_defined.
+Qed.
+
+Global Instance Proper_equivalent_behaviour_exact_equivalence :
+  Proper
+    (exact_equivalence ==> exact_equivalence ==> iff)
+    (equivalent_behaviour).
+Proof.
+  intros v1 v2 Heq v1' v2' Heq'. split; intro Heq_behaviour.
+  - constructor.
+    + destruct Heq, Heq', Heq_behaviour. congruence.
+    + destruct Heq, Heq', Heq_behaviour. congruence.
+    + destruct Heq_behaviour.
+      eapply transfer_clean; eassumption.
+    + destruct Heq_behaviour.
+      eapply transfer_clean; eassumption.
+    + destruct Heq, Heq', Heq_behaviour.
+      setoid_rewrite <- execution_match0.
+      setoid_rewrite <- execution_match1.
+      setoid_rewrite <- inputs_same0.
+      setoid_rewrite <- outputs_same0.
+      assumption.
+  - constructor.
+    + destruct Heq, Heq', Heq_behaviour. congruence.
+    + destruct Heq, Heq', Heq_behaviour. congruence.
+    + destruct Heq_behaviour.
+      eapply transfer_clean; try symmetry; eassumption.
+    + inv Heq_behaviour.
+      eapply transfer_clean; try symmetry; eassumption.
+    + destruct Heq, Heq', Heq_behaviour.
+      setoid_rewrite execution_match0.
+      setoid_rewrite execution_match1.
+      setoid_rewrite inputs_same0.
+      setoid_rewrite outputs_same0.
+      assumption.
+Qed.
+
+Theorem equivalence_query_general_unsat_correct v1 v2 smt :
+  equivalence_query_general v1 v2 = inr smt ->
+  (forall ρ, ~ satisfied_by ρ (SMT.query smt)) ->
+  equivalent_behaviour v1 v2.
+Proof.
+  unfold equivalence_query_general.
+  intros. monad_inv.
+  do 2 apply_somewhere AssignmentForwardingCorrect.assignment_forwarding_exact_equivalence.
+  do 2 apply_somewhere sort_module_equivalent.
+  do 2 apply_somewhere DropInternal.drop_internal_correct.
+  apply_somewhere VerilogEquivalenceCorrectness.equivalence_query_unsat_correct; [|eassumption].
+  repeat match goal with
+         | [ H : ?l ~~~ ?l' |- ?l ~~ ?r ] => rewrite H; clear H
+         | [ H : ?r ~~~ ?r' |- ?l ~~ ?r ] => rewrite H; clear H
+	 end.
+  assumption.
+Qed.
+
+Lemma counterexample_transfer v1 v2 v1' v2' e1 e2 :
+  v1 ~~~ v1' ->
+  v2 ~~~ v2' ->
+  counterexample_execution v1 e1 v2 e2 ->
+  counterexample_execution v1' e1 v2' e2.
+Proof.
+  intros [] [] Hcounterexample.
+  unfold counterexample_execution in *.
+  rewrite <- execution_match0.
+  rewrite <- execution_match1.
+  rewrite <- inputs_same0.
+  rewrite <- outputs_same0.
+  assumption.
+Qed.
+
+Global Instance Proper_counterexample_execution_exact_equivalence :
+  Proper
+    (exact_equivalence ==> eq ==> exact_equivalence ==> eq ==> iff)
+    counterexample_execution.
+Proof.
+  repeat intro; subst; split; intro.
+  - eapply counterexample_transfer; eauto.
+  - eapply counterexample_transfer; (symmetry + idtac); eauto.
+Qed.
+
+Theorem equivalence_query_general_sat_correct v1 v2 smt ρ :
+  equivalence_query_general v1 v2 = inr smt ->
+  satisfied_by ρ (SMT.query smt) ->
+  exists e1 e2, counterexample_execution v1 e1 v2 e2.
+Proof.
+  intros. unfold equivalence_query_general in *. monad_inv.
+  do 2 apply_somewhere AssignmentForwardingCorrect.assignment_forwarding_exact_equivalence.
+  do 2 apply_somewhere sort_module_equivalent.
+  do 2 apply_somewhere DropInternal.drop_internal_correct.
+  repeat match goal with
+         | [ H : ?l ~~~ ?l' |- context[?l] ] => setoid_rewrite H; clear H
+	 end.
+  eexists. eexists.
+  eapply equivalence_query_sat_correct; eassumption.
+Qed.
+
+Print Assumptions equivalence_query_general_unsat_correct.
+Print Assumptions equivalence_query_general_sat_correct.
